some renaming and refactoring

messageInvariantPrototypes/shardedKv/distributedMonotonic/ownershipInvariants.dfy
@@ -5,76 +5,87 @@ module OwnershipInvariants {
   import opened UtilitiesLibrary
   import opened DistributedSystem
 
-  ghost predicate KeyInFlight(c: Constants, v: Variables, k: OwnedKey) 
+/***************************************************************************************
+*                                   Definitions                                        *
+***************************************************************************************/
+
+  ghost predicate UniqueKeyInFlight(c: Constants, v: Variables, k: UniqueKey) 
     requires v.WF(c)
   {
     exists msg :: KeyInFlightByMessage(c, v, msg, k)
   }
 
-  ghost predicate KeyInFlightByMessage(c: Constants, v: Variables, msg: Message, k: OwnedKey) 
+  ghost predicate KeyInFlightByMessage(c: Constants, v: Variables, msg: Message, k: UniqueKey) 
     requires v.WF(c)
   {
     && msg in v.network.sentMsgs
     && (0 <= msg.Dst() < |c.hosts| ==>
-      Host.OwnedKeyInFlight(c.hosts[msg.Dst()], v.Last().hosts[msg.Dst()], k, msg)
+      Host.UniqueKeyInFlight(c.hosts[msg.Dst()], v.Last().hosts[msg.Dst()], k, msg)
     )
   }
 
-  ghost predicate AtMostOneInFlight(c: Constants, v: Variables)
+  ghost predicate NoHostOwnsKey(c: Constants, v: Variables, k: UniqueKey) 
+    requires v.WF(c)
+  {
+    forall idx | c.ValidIdx(idx) :: !Host.HostOwnsUniqueKey(c.hosts[idx], v.Last().hosts[idx], k)
+  }
+
+/***************************************************************************************
+*                                    Invariants                                        *
+***************************************************************************************/
+
+
+  ghost predicate AtMostOneInFlightMessagePerKey(c: Constants, v: Variables)
     requires v.WF(c)
   {
     forall k, m1, m2 | KeyInFlightByMessage(c, v, m1, k) && KeyInFlightByMessage(c, v, m2, k) 
     :: m1 == m2
   }
 
-  ghost predicate NoHostOwnsKey(c: Constants, v: Variables, k: OwnedKey) 
-    requires v.WF(c)
-  {
-    forall idx | c.ValidIdx(idx) :: !Host.HostOwnsKey(c.hosts[idx], v.Last().hosts[idx], k)
-  }
-
-  ghost predicate HostOwnsKeyImpliesNoneInFlight(c: Constants, v: Variables)
+  ghost predicate HostOwnsKeyImpliesNotInFlight(c: Constants, v: Variables)
     requires v.WF(c)
   {
     forall k | !NoHostOwnsKey(c, v, k)
     ::
-    !KeyInFlight(c, v, k)
+    !UniqueKeyInFlight(c, v, k)
   }
 
-  ghost predicate AtMostOwnedByOneHost(c: Constants, v: Variables)
+  ghost predicate AtMostOwnerPerKey(c: Constants, v: Variables)
     requires v.WF(c)
   {
     forall h1, h2, k | 
       && c.ValidIdx(h1) 
       && c.ValidIdx(h2)
-      && Host.HostOwnsKey(c.hosts[h1], v.Last().hosts[h1], k) 
-      && Host.HostOwnsKey(c.hosts[h2], v.Last().hosts[h2], k) 
+      && Host.HostOwnsUniqueKey(c.hosts[h1], v.Last().hosts[h1], k) 
+      && Host.HostOwnsUniqueKey(c.hosts[h2], v.Last().hosts[h2], k) 
     ::
      h1 == h2
   }
-
+  
   
   ghost predicate OwnershipInv(c: Constants, v: Variables)
   {
     && v.WF(c)
-    && AtMostOneInFlight(c, v)
-    && AtMostOwnedByOneHost(c, v)
-    && HostOwnsKeyImpliesNoneInFlight(c, v)
+    && AtMostOneInFlightMessagePerKey(c, v)
+    && AtMostOwnerPerKey(c, v)
+    && HostOwnsKeyImpliesNotInFlight(c, v)
   }
 
+  // Base obligation
   lemma InitImpliesOwnershipInv(c: Constants, v: Variables)
     requires Init(c, v)
     ensures OwnershipInv(c, v)
   {}
 
+  // Inductive obligation
   lemma OwnershipInvInductive(c: Constants, v: Variables, v': Variables)
     requires OwnershipInv(c, v)
     requires Next(c, v, v')
     ensures OwnershipInv(c, v')
   {
-    InvNextAtMostOneInFlight(c, v, v');
-    InvNextLiveKeyImpliesNoneInFlight(c, v, v');
-    InvNextAtMostOwnedByOneHost(c, v, v');
+    InvNextAtMostOneInFlightMessagePerKey(c, v, v');
+    InvNextHostOwnsKeyImpliesNotInFlight(c, v, v');
+    InvNextAtMostOwnerPerKey(c, v, v');
   }
 
 
@@ -83,11 +94,11 @@ module OwnershipInvariants {
 ***************************************************************************************/
 
 
-lemma InvNextAtMostOneInFlight(c: Constants, v: Variables, v': Variables)
+lemma InvNextAtMostOneInFlightMessagePerKey(c: Constants, v: Variables, v': Variables)
   requires v'.WF(c)
   requires OwnershipInv(c, v)
   requires Next(c, v, v')
-  ensures AtMostOneInFlight(c, v')
+  ensures AtMostOneInFlightMessagePerKey(c, v')
 {
   forall k, m1, m2 | KeyInFlightByMessage(c, v', m1, k) && KeyInFlightByMessage(c, v', m2, k) 
   ensures m1 == m2
@@ -102,7 +113,7 @@ lemma InvNextAtMostOneInFlight(c: Constants, v: Variables, v': Variables)
   }
 }
 
-lemma InvNextAtMostOneInFlightHelper(c: Constants, v: Variables, v': Variables, m1: Message, m2: Message, k: OwnedKey)
+lemma InvNextAtMostOneInFlightHelper(c: Constants, v: Variables, v': Variables, m1: Message, m2: Message, k: UniqueKey)
   requires v'.WF(c)
   requires OwnershipInv(c, v)
   requires Next(c, v, v')
@@ -113,24 +124,24 @@ lemma InvNextAtMostOneInFlightHelper(c: Constants, v: Variables, v': Variables, 
   // postcondition
   ensures !KeyInFlightByMessage(c, v', m2, k)
 {
-  assert KeyInFlight(c, v, k);
+  assert UniqueKeyInFlight(c, v, k);
 }
 
-lemma InvNextLiveKeyImpliesNoneInFlight(c: Constants, v: Variables, v': Variables)
+lemma InvNextHostOwnsKeyImpliesNotInFlight(c: Constants, v: Variables, v': Variables)
   requires v'.WF(c)
   requires OwnershipInv(c, v)
   requires Next(c, v, v')
-  ensures HostOwnsKeyImpliesNoneInFlight(c, v')
+  ensures HostOwnsKeyImpliesNotInFlight(c, v')
 {
   forall k | !NoHostOwnsKey(c, v', k)
-  ensures !KeyInFlight(c, v', k)
+  ensures !UniqueKeyInFlight(c, v', k)
   {
     forall msg | msg in v'.network.sentMsgs
     ensures !KeyInFlightByMessage(c, v', msg, k) {
-      var idx :| c.ValidIdx(idx) && Host.HostOwnsKey(c.hosts[idx], v'.Last().hosts[idx], k);
-      if Host.HostOwnsKey(c.hosts[idx], v.Last().hosts[idx], k){
+      var idx :| c.ValidIdx(idx) && Host.HostOwnsUniqueKey(c.hosts[idx], v'.Last().hosts[idx], k);
+      if Host.HostOwnsUniqueKey(c.hosts[idx], v.Last().hosts[idx], k){
         // triggers
-        assert !KeyInFlight(c, v, k);
+        assert !UniqueKeyInFlight(c, v, k);
         assert !KeyInFlightByMessage(c, v, msg, k);
 
       } else {
@@ -138,7 +149,7 @@ lemma InvNextLiveKeyImpliesNoneInFlight(c: Constants, v: Variables, v': Variable
           var dsStep :| NextStep(c, v.Last(), v'.Last(), v.network, v'.network, dsStep);
           // triggers
           assert KeyInFlightByMessage(c, v, dsStep.msgOps.recv.value, k);
-          assert KeyInFlight(c, v, k);
+          assert UniqueKeyInFlight(c, v, k);
         }
         assert !KeyInFlightByMessage(c, v', msg, k);
       }
@@ -146,17 +157,17 @@ lemma InvNextLiveKeyImpliesNoneInFlight(c: Constants, v: Variables, v': Variable
   }
 }
 
-lemma InvNextAtMostOwnedByOneHost(c: Constants, v: Variables, v': Variables) 
+lemma InvNextAtMostOwnerPerKey(c: Constants, v: Variables, v': Variables) 
   requires v'.WF(c)
   requires OwnershipInv(c, v)
   requires Next(c, v, v')
-  ensures AtMostOwnedByOneHost(c, v')
+  ensures AtMostOwnerPerKey(c, v')
 {
   forall h1, h2, k | 
       && c.ValidIdx(h1) 
       && c.ValidIdx(h2)
-      && Host.HostOwnsKey(c.hosts[h1], v'.Last().hosts[h1], k) 
-      && Host.HostOwnsKey(c.hosts[h2], v'.Last().hosts[h2], k) 
+      && Host.HostOwnsUniqueKey(c.hosts[h1], v'.Last().hosts[h1], k) 
+      && Host.HostOwnsUniqueKey(c.hosts[h2], v'.Last().hosts[h2], k) 
   ensures
      h1 == h2
   {
@@ -170,27 +181,26 @@ lemma InvNextAtMostOwnedByOneHost(c: Constants, v: Variables, v': Variables)
   }
 }
 
-
-lemma AtMostOneHostOwnsKey(c: Constants, v: Variables, v': Variables, k: OwnedKey, idx: HostId, other: HostId)
+lemma AtMostOneHostOwnsKey(c: Constants, v: Variables, v': Variables, k: UniqueKey, idx: HostId, other: HostId)
   requires v.WF(c) && v'.WF(c)
   requires OwnershipInv(c, v)
   requires c.ValidIdx(idx)
   requires c.ValidIdx(other)
   requires idx != other
-  requires Host.HostOwnsKey(c.hosts[idx], v.Last().hosts[idx], k) 
-  requires !Host.HostOwnsKey(c.hosts[other], v.Last().hosts[other], k) 
+  requires Host.HostOwnsUniqueKey(c.hosts[idx], v.Last().hosts[idx], k) 
+  requires !Host.HostOwnsUniqueKey(c.hosts[other], v.Last().hosts[other], k) 
   requires Next(c, v, v')
-  ensures !Host.HostOwnsKey(c.hosts[other], v'.Last().hosts[other], k) 
+  ensures !Host.HostOwnsUniqueKey(c.hosts[other], v'.Last().hosts[other], k) 
 {
   var dsStep :| NextStep(c, v.Last(), v'.Last(), v.network, v'.network, dsStep);
   var actor, msgOps := dsStep.actor, dsStep.msgOps;
   if actor == other {
     var cs, s, s' := c.hosts[other], v.Last().hosts[other], v'.Last().hosts[other];
     var step :| Host.NextStep(cs, s, s', step, msgOps);
-    if step.ReceiveStep? && Host.HostOwnsKey(c.hosts[other], v'.Last().hosts[other], k) {
+    if step.ReceiveStep? && Host.HostOwnsUniqueKey(c.hosts[other], v'.Last().hosts[other], k) {
       // triggers
       assert KeyInFlightByMessage(c, v, msgOps.recv.value, k);  
-      assert KeyInFlight(c, v, k);
+      assert UniqueKeyInFlight(c, v, k);
       assert false;
     }    
   }
