messageInvariantPrototypes/shardedKv/types.dfy
@@ -4,10 +4,10 @@ module Types {
   import opened UtilitiesLibrary
 
   type HostId = nat
-  type OwnedKey = int
+  type UniqueKey = int
   datatype Entry = Entry(live: bool, version: nat)
 
-  datatype Message = Reconf(src: nat, dst: nat, key: OwnedKey, version: nat) {
+  datatype Message = Reconf(src: nat, dst: nat, key: UniqueKey, version: nat) {
     function Src() : nat {
       src
     }
